src/coq/Semantics/Memory/ErrSID.v
@@ -16,7 +16,8 @@ From Vellvm Require Import
      Semantics.Memory.FiniteProvenance
      Semantics.Memory.Sizeof
      Utils.StateMonads
-     Utils.Monads.
+     Utils.Monads
+     Utils.MonadExcLaws.
 
 From ITree Require Import
      ITree
@@ -25,6 +26,8 @@ From ITree Require Import
      Eq.Eq
      Events.StateFacts
      Events.State.
+
+Import Morphisms.
 
 Import Basics.Basics.Monads.
 
@@ -71,8 +74,11 @@ Module ERRSID (Addr:ADDRESS) (IP:INTPTR) (SIZEOF:Sizeof) (LLVMEvents:LLVM_INTERA
   Definition runErrSID {A} (m : ErrSID A) (sid : store_id) (prov : Provenance) : (OOM_MESSAGE + UB (ERR A)) * store_id * Provenance%type
     := unIdent (runErrSID_T m sid prov).
 
-  Definition ErrSID_evals_to {A} (e : ErrSID A) (x : A) sid pr : Prop
+  Definition ErrSID_evals_to {A} (e : ErrSID A) sid pr (x : A) : Prop
     := evalErrSID e sid pr = inr (inr (inr x)).
+
+  Definition ErrSID_runs_to {A} (e : ErrSID A) sid pr (x : A) sid' pr': Prop
+    := runErrSID e sid pr = (inr (inr (inr x)), sid', pr').
 
   Definition fresh_sid : ErrSID store_id
     := lift (lift (modify N.succ)).
@@ -90,5 +96,149 @@ Module ERRSID (Addr:ADDRESS) (IP:INTPTR) (SIZEOF:Sizeof) (LLVMEvents:LLVM_INTERA
            raise_ub msg
        | inr x => ret x
        end.
+
+  Section Lemmas.
+    Lemma ErrSID_evals_to_bind :
+      forall {A X} sid prov (m : ErrSID X) k (res : A),
+        ErrSID_evals_to (bind m k) sid prov res ->
+        exists sid' prov' x,
+          ErrSID_runs_to m sid prov x sid' prov' /\
+            ErrSID_evals_to (k x) sid' prov' res.
+    Proof.
+      intros A X sid prov m k res EVAL.
+      
+      cbn in EVAL.
+      inversion EVAL as [EVAL'].
+      clear EVAL.
+      rename EVAL' into EVAL.
+      cbn in EVAL.
+
+      unfold ErrSID_runs_to.
+      unfold runErrSID.
+      cbn.
+
+      destruct (IdentityMonad.unIdent (unEitherT (unEitherT (unEitherT m)) sid prov)) as (p, p0) eqn:BLAH.
+      destruct p0.
+      cbn in *.
+
+      destruct s0; cbn in *; inversion EVAL.
+      destruct s0; cbn in *; inversion EVAL.
+      destruct s0; cbn in *; inversion EVAL.
+
+      do 3 eexists.
+      split.
+      { 
+        reflexivity.
+      }
+      {
+        unfold ErrSID_evals_to.
+        cbn.
+        auto.
+      }
+    Qed.
+
+    Lemma ErrSID_runs_to_bind :
+      forall {A X} sid prov (m : ErrSID X) k (res : A) sid_final prov_final,
+        ErrSID_runs_to (bind m k) sid prov res sid_final prov_final ->
+        exists sid' prov' x,
+          ErrSID_runs_to m sid prov x sid' prov' /\
+            ErrSID_runs_to (k x) sid' prov' res sid_final prov_final.
+    Proof.
+      intros A X sid prov m k res sid_final prov_final EVAL.
+      
+      cbn in EVAL.
+      inversion EVAL as [EVAL'].
+      clear EVAL.
+      rename EVAL' into EVAL.
+      cbn in EVAL.
+
+      unfold ErrSID_runs_to.
+      unfold runErrSID in *.
+      cbn.
+
+      destruct (IdentityMonad.unIdent (unEitherT (unEitherT (unEitherT m)) sid prov)) as (p, p0) eqn:BLAH.
+      destruct p0.
+      cbn in *.
+      rewrite BLAH in EVAL.
+
+      destruct s0; cbn in *; inversion EVAL.
+      destruct s0; cbn in *; inversion EVAL.
+      destruct s0; cbn in *; inversion EVAL.
+
+      do 3 eexists.
+      split.
+      { 
+        reflexivity.
+      }
+      {
+        unfold ErrSID_evals_to.
+        cbn.
+        auto.
+      }
+    Qed.
+
+    Lemma ErrSID_runs_to_ErrSID_evals_to :
+      forall {X} sid prov sid' prov' (m : ErrSID X) (res : X),
+        ErrSID_runs_to m sid prov res sid' prov' ->
+        ErrSID_evals_to m sid prov res.
+    Proof.
+      intros X sid prov sid' prov' m res H.
+      unfold ErrSID_runs_to in H.
+      unfold ErrSID_evals_to.
+      cbn.
+      unfold runErrSID in H.
+      cbn in H.
+      match goal with
+      |  H: _ |- fst (snd ?x) = _
+         => destruct x
+      end.
+      cbn in H.
+      inversion H.
+      reflexivity.
+    Qed.
+
+    Global Instance proper_eq1_runs_to : forall {A}, Proper (@Monad.eq1 (eitherT ERR_MESSAGE (eitherT UB_MESSAGE _)) _ A ==> eq ==> eq ==> eq ==> eq  ==> eq ==> iff) (ErrSID_runs_to).
+    Proof.
+      repeat intro; subst. rename H into EQ.
+
+      unfold Monad.eq1, Eq1_eitherT in EQ.
+      split; intros RUNS.
+      - unfold Monad.eq1 in EQ.
+        unfold MonadState.Eq1_stateTM in EQ.
+        unfold pointwise_relation in EQ.
+        unfold Monad.eq1 in EQ.
+        unfold Eq1_ident in EQ.
+
+        cbn in EQ.
+        unfold unEitherT in EQ.
+        destruct x as [x].
+        destruct y as [y].
+        destruct x as [x].
+        destruct y as [y].
+
+        unfold ErrSID_runs_to, runErrSID, runErrSID_T in *.
+        cbn in *.
+        rewrite <- EQ.
+        auto.
+      - unfold Monad.eq1 in EQ.
+        unfold MonadState.Eq1_stateTM in EQ.
+        unfold pointwise_relation in EQ.
+        unfold Monad.eq1 in EQ.
+        unfold Eq1_ident in EQ.
+
+        cbn in EQ.
+        unfold unEitherT in EQ.
+        destruct x as [x].
+        destruct y as [y].
+        destruct x as [x].
+        destruct y as [y].
+
+        unfold ErrSID_runs_to, runErrSID, runErrSID_T in *.
+        cbn in *.
+        rewrite EQ.
+        auto.
+    Qed.
+
+  End Lemmas.
 
 End ERRSID.
